theories/iris/logrel/fundamental.v
@@ -1,56 +1,10 @@
-From mathcomp Require Import ssreflect ssrbool eqtype seq.
-
-From stdpp Require Import base fin_maps option list.
-
-From ExtLib.Structures Require Import Monads.
-From ExtLib.Data.Monads Require Import StateMonad.
-
-From iris.program_logic Require Import language.
-From iris.proofmode Require Import base tactics classes.
-From iris.base_logic Require Export gen_heap ghost_map proph_map na_invariants.
-From iris.base_logic.lib Require Export fancy_updates.
-From iris.algebra Require Import list.
-From iris.prelude Require Import options.
-
-From RichWasm.iris.helpers Require Export iris_properties.
-From RichWasm.iris.language Require Export iris_atomicity lenient_wp lwp_pure lwp_structural lwp_resources lwp_trap.
-From RichWasm.iris.rules Require Export iris_rules.
-
 From RichWasm Require Import syntax typing.
 From RichWasm.compiler Require Import codegen instrs modules util.
 From RichWasm.iris Require Import autowp gc.
 From RichWasm.iris.logrel Require Import relations.
-Require Import RichWasm.util.
-
-Module RT := RichWasm.syntax.
-Module T := RichWasm.typing.
-
-Import uPred.
 
 Set Bullet Behavior "Strict Subproofs".
-Set Default Goal Selector "1".
-
-Ltac fill_vals_pred' vs :=
-  instantiate ( 1 := (λ w, ⌜w = vs⌝ ∗ _)%I).
-
-Ltac curry_hyps :=
-  iRevert "∗";
-  rewrite ? wand_curry.
-
-Ltac fill_goal :=
-  match goal with
-  | |- environments.envs_entails _ ?E =>
-      is_evar E;
-      curry_hyps;
-      try (iApply wand_refl; solve_constraints);
-      instantiate (1:= ⌜True⌝%I); done
-  end.
-
-Ltac fill_vals_pred :=
-  match goal with
-  | |- environments.envs_entails _ (?g ?vs) =>
-      fill_vals_pred' vs; iSplitR; [done | fill_goal]
-  end.
+Set Default Goal Selector "!".
 
 Section Fundamental.
 
@@ -59,20 +13,599 @@ Section Fundamental.
   Context `{!RichWasmGCG Σ}.
 
   Variable sr : store_runtime.
+  Variable mr : module_runtime.
 
-  Theorem fundamental_property M F L L' me fe es es' tf wl wl' :
+  Lemma compat_nop M F L wl wl' es' :
+    let me := me_of_context M mr in
+    let fe := fe_of_context F in
+    let ψ := ArrowT [] [] in
+    run_codegen (compile_instr me fe (INop ψ)) wl = inr ((), wl', es') ->
+    ⊢ has_type_semantic sr M F L [] (to_e_list es') ψ L.
+  Admitted.
+
+  Lemma compat_unreachable M F L L' wl wl' τs1 τs2 es' :
+    let me := me_of_context M mr in
+    let fe := fe_of_context F in
+    let ψ := ArrowT τs1 τs2 in
+    run_codegen (compile_instr me fe (IUnreachable ψ)) wl = inr ((), wl', es') ->
+    ⊢ has_type_semantic sr M F L [] (to_e_list es') ψ L'.
+  Admitted.
+
+  Lemma compat_copy M F L wl wl' τ es' :
+    let me := me_of_context M mr in
+    let fe := fe_of_context F in
+    has_copyability F τ ExCopy ->
+    let ψ := ArrowT [τ] [τ; τ] in
+    run_codegen (compile_instr me fe (ICopy ψ)) wl = inr ((), wl', es') ->
+    ⊢ has_type_semantic sr M F L [] (to_e_list es') ψ L.
+  Admitted.
+
+  Lemma compat_drop M F L wl wl' τ es' :
+    let me := me_of_context M mr in
+    let fe := fe_of_context F in
+    has_dropability F τ ExDrop ->
+    let ψ := ArrowT [τ] [] in
+    run_codegen (compile_instr me fe (IDrop ψ)) wl = inr ((), wl', es') ->
+    ⊢ has_type_semantic sr M F L [] (to_e_list es') ψ L.
+  Admitted.
+
+  Lemma compat_num M F L wl wl' ψ eₙ es' :
+    let me := me_of_context M mr in
+    let fe := fe_of_context F in
+    num_instr_has_type eₙ ψ ->
+    run_codegen (compile_instr me fe (INum ψ eₙ)) wl = inr ((), wl', es') ->
+    ⊢ has_type_semantic sr M F L [] (to_e_list es') ψ L.
+  Admitted.
+
+  Lemma compat_num_const M F L wl wl' n ν κ es' :
+    let me := me_of_context M mr in
+    let fe := fe_of_context F in
+    has_kind F (NumT κ ν) κ ->
+    let ψ := ArrowT [] [NumT κ ν] in
+    run_codegen (compile_instr me fe (INumConst ψ n)) wl = inr ((), wl', es') ->
+    ⊢ has_type_semantic sr M F L [] (to_e_list es') ψ L.
+  Admitted.
+
+  Lemma compat_block M F L wl wl' ξ τs1 τs2 es es' :
+    let me := me_of_context M mr in
+    let fe := fe_of_context F in
+    let L' := update_locals ξ L in
+    let F' := RecordSet.set fc_labels (cons (τs2, L')) F in
+    let ψ := ArrowT τs1 τs2 in
+    instrs_have_type M F' L es ψ L' ->
+    (forall wl wl' es',
+        let fe' := fe_of_context F' in
+        run_codegen (compile_instrs me fe' es) wl = inr ((), wl', es') ->
+        ⊢ has_type_semantic sr M F' L wl' (to_e_list es') ψ L') ->
+    run_codegen (compile_instr me fe (IBlock ψ ξ es)) wl = inr ((), wl', es') ->
+    ⊢ has_type_semantic sr M F L [] (to_e_list es') ψ L'.
+  Admitted.
+
+  Lemma compat_loop M F L wl wl' es es' τs1 τs2 :
+    let me := me_of_context M mr in
+    let fe := fe_of_context F in
+    let F' := RecordSet.set fc_labels (cons (τs1, L)) F in
+    let ψ := ArrowT τs1 τs2 in
+    instrs_have_type M F' L es ψ L ->
+    (forall wl wl' es',
+        let fe' := fe_of_context F' in
+        run_codegen (compile_instrs me fe' es) wl = inr ((), wl', es') ->
+        ⊢ has_type_semantic sr M F' L wl' (to_e_list es') ψ L) ->
+    run_codegen (compile_instr me fe (ILoop ψ es)) wl = inr ((), wl', es') ->
+    ⊢ has_type_semantic sr M F L [] (to_e_list es') ψ L.
+  Admitted.
+
+  Lemma compat_ite M F L wl wl' es1 es2 es' ξ ψ :
+    let me := me_of_context M mr in
+    let fe := fe_of_context F in
+    let L' := update_locals ξ L in
+    instrs_have_type M F L es1 ψ L' ->
+    instrs_have_type M F L es2 ψ L' ->
+    (forall wl wl' es',
+        run_codegen (compile_instrs me fe es1) wl = inr ((), wl', es') ->
+        ⊢ has_type_semantic sr M F L wl' (to_e_list es') ψ L') ->
+    (forall wl wl' es',
+        run_codegen (compile_instrs me fe es2) wl = inr ((), wl', es') ->
+        ⊢ has_type_semantic sr M F L wl' (to_e_list es') ψ L') ->
+    run_codegen (compile_instr me fe (IIte ψ ξ es1 es2)) wl = inr ((), wl', es') ->
+    ⊢ has_type_semantic sr M F L [] (to_e_list es') ψ L'.
+  Admitted.
+
+  Lemma compat_br M F L wl wl' es' n τs1 τs τs2 ξ :
+    let me := me_of_context M mr in
+    let fe := fe_of_context F in
+    fc_labels F !! n = Some (τs, L) ->
+    Forall (fun τ => has_dropability F τ ImDrop) τs1 ->
+    let ψ := ArrowT (τs1 ++ τs) τs2 in
+    let L' := update_locals ξ L in
+    run_codegen (compile_instr me fe (IBr ψ n)) wl = inr ((), wl', es') ->
+    ⊢ has_type_semantic sr M F L [] (to_e_list es') ψ L'.
+  Admitted.
+
+  Lemma compat_br_if M F L wl wl' es' n τs κ :
+    let me := me_of_context M mr in
+    let fe := fe_of_context F in
+    fc_labels F !! n = Some (τs, L) ->
+    let τ := NumT κ (IntT I32T) in
+    has_kind F τ κ ->
+    let ψ := ArrowT (τs ++ [τ]) τs in
+    run_codegen (compile_instr me fe (IBrIf ψ n)) wl = inr ((), wl', es') ->
+    ⊢ has_type_semantic sr M F L [] (to_e_list es') ψ L.
+  Admitted.
+
+  Lemma compat_br_table M F L L' wl wl' es' n ns τs τs1 τs2 κ :
+    let me := me_of_context M mr in
+    let fe := fe_of_context F in
+    Forall (fun i => fc_labels F !! i = Some (τs, L)) (n :: ns) ->
+    Forall (fun τ => has_dropability F τ ImDrop) τs1 ->
+    let τ := NumT κ (IntT I32T) in
+    has_kind F τ κ ->
+    let ψ := ArrowT (τs1 ++ τs ++ [τ]) τs2 in
+    run_codegen (compile_instr me fe (IBrTable ψ ns n)) wl = inr ((), wl', es') ->
+    ⊢ has_type_semantic sr M F L [] (to_e_list es') ψ L'.
+  Admitted.
+
+  Lemma compat_return M F L L' wl wl' es' τs τs1 τs2 :
+    let me := me_of_context M mr in
+    let fe := fe_of_context F in
+    fc_return_type F = τs ->
+    Forall (fun τ => has_dropability F τ ImDrop) τs1 ->
+    let ψ := ArrowT (τs1 ++ τs) τs2 in
+    run_codegen (compile_instr me fe (IReturn ψ)) wl = inr ((), wl', es') ->
+    ⊢ has_type_semantic sr M F L [] (to_e_list es') ψ L'.
+  Admitted.
+
+  Lemma compat_local_get M F L wl wl' es' n τ ρ κ κ0 :
+    let me := me_of_context M mr in
+    let fe := fe_of_context F in
+    L !! n = Some τ ->
+    has_rep F τ ρ ->
+    let τ' := RepT κ ρ (ProdT κ0 []) in
+    has_kind F τ' κ ->
+    let L' := <[n := τ']> L in
+    let ψ := ArrowT [] [τ] in
+    run_codegen (compile_instr me fe (ILocalGet ψ n)) wl = inr ((), wl', es') ->
+    ⊢ has_type_semantic sr M F L [] (to_e_list es') ψ L'.
+  Admitted.
+
+  Lemma compat_local_get_copy M F L wl wl' es' n τ :
+    let me := me_of_context M mr in
+    let fe := fe_of_context F in
+    L !! n = Some τ ->
+    has_copyability F τ ImCopy ->
+    let ψ := ArrowT [] [τ] in
+    run_codegen (compile_instr me fe (ILocalGet ψ n)) wl = inr ((), wl', es') ->
+    ⊢ has_type_semantic sr M F L [] (to_e_list es') ψ L.
+  Admitted.
+
+  Lemma compat_local_set M F L wl wl' es' n τ τ' ρ :
+    let me := me_of_context M mr in
+    let fe := fe_of_context F in
+    L !! n = Some τ ->
+    has_dropability F τ ImDrop ->
+    has_rep F τ ρ ->
+    has_rep F τ' ρ ->
+    let L' := <[n := τ']> L in
+    let ψ := ArrowT [τ'] [] in
+    run_codegen (compile_instr me fe (ILocalSet ψ n)) wl = inr ((), wl', es') ->
+    ⊢ has_type_semantic sr M F L [] (to_e_list es') ψ L'.
+  Admitted.
+
+  Lemma compat_global_get M F L wl wl' es' n m τ :
+    let me := me_of_context M mr in
+    let fe := fe_of_context F in
+    mc_globals M !! n = Some (m, τ) ->
+    has_copyability F τ ImCopy ->
+    let ψ := ArrowT [] [τ] in
+    run_codegen (compile_instr me fe (IGlobalGet ψ n)) wl = inr ((), wl', es') ->
+    ⊢ has_type_semantic sr M F L [] (to_e_list es') ψ L.
+  Admitted.
+
+  Lemma compat_global_set M F L wl wl' es' n τ :
+    let me := me_of_context M mr in
+    let fe := fe_of_context F in
+    mc_globals M !! n = Some (Mut, τ) ->
+    has_dropability F τ ImDrop ->
+    let ψ := ArrowT [τ] [] in
+    run_codegen (compile_instr me fe (IGlobalSet ψ n)) wl = inr ((), wl', es') ->
+    ⊢ has_type_semantic sr M F L [] (to_e_list es') ψ L.
+  Admitted.
+
+  Lemma compat_global_swap M F L wl wl' es' n τ :
+    let me := me_of_context M mr in
+    let fe := fe_of_context F in
+    mc_globals M !! n = Some (Mut, τ) ->
+    let ψ := ArrowT [τ] [τ] in
+    run_codegen (compile_instr me fe (IGlobalSwap ψ n)) wl = inr ((), wl', es') ->
+    ⊢ has_type_semantic sr M F L [] (to_e_list es') ψ L.
+  Admitted.
+
+  Lemma compat_coderef M F L wl wl' es' i ϕ κ :
+    let me := me_of_context M mr in
+    let fe := fe_of_context F in
+    mc_table M !! i = Some ϕ ->
+    let τ := CodeRefT κ ϕ in
+    has_kind F τ κ ->
+    let ψ := ArrowT [] [τ] in
+    run_codegen (compile_instr me fe (ICodeRef ψ i)) wl = inr ((), wl', es') ->
+    ⊢ has_type_semantic sr M F L [] (to_e_list es') ψ L.
+  Admitted.
+
+  Lemma compat_inst M F L wl wl' es' ix ϕ ϕ' κ :
+    let me := me_of_context M mr in
+    let fe := fe_of_context F in
+    inst_function_type F ix ϕ ϕ' ->
+    let ψ := ArrowT [CodeRefT κ ϕ] [CodeRefT κ ϕ'] in
+    run_codegen (compile_instr me fe (IInst ψ ix)) wl = inr ((), wl', es') ->
+    ⊢ has_type_semantic sr M F L [] (to_e_list es') ψ L.
+  Admitted.
+
+  Lemma compat_call M F L wl wl' es' i ixs ϕ τs1 τs2 :
+    let me := me_of_context M mr in
+    let fe := fe_of_context F in
+    mc_table M !! i = Some ϕ ->
+    let ψ := ArrowT τs1 τs2 in
+    list_inst_function_type F ixs ϕ (FunT ψ) ->
+    run_codegen (compile_instr me fe (ICall ψ i ixs)) wl = inr ((), wl', es') ->
+    ⊢ has_type_semantic sr M F L [] (to_e_list es') ψ L.
+  Admitted.
+
+  Lemma compat_call_indirect M F L wl wl' es' τs1 τs2 κ :
+    let me := me_of_context M mr in
+    let fe := fe_of_context F in
+    let ψ := ArrowT (τs1 ++ [CodeRefT κ (FunT (ArrowT τs1 τs2))]) τs2 in
+    run_codegen (compile_instr me fe (ICallIndirect ψ)) wl = inr ((), wl', es') ->
+    ⊢ has_type_semantic sr M F L [] (to_e_list es') ψ L.
+  Admitted.
+
+  Lemma compat_inject M F L wl wl' es' i τs τ κ :
+    let me := me_of_context M mr in
+    let fe := fe_of_context F in
+    τs !! i = Some τ ->
+    let ψ := ArrowT [τ] [SumT κ τs] in
+    run_codegen (compile_instr me fe (IInject ψ i)) wl = inr ((), wl', es') ->
+    ⊢ has_type_semantic sr M F L [] (to_e_list es') ψ L.
+  Admitted.
+
+  Lemma compat_case M F L wl wl' es' ξ ess τ' τs κ :
+    let me := me_of_context M mr in
+    let fe := fe_of_context F in
+    let L' := update_locals ξ L in
+    Forall2 (fun τ es => instrs_have_type M F L es (ArrowT [τ] [τ']) L') τs ess ->
+    let ψ := ArrowT [SumT κ τs] [τ'] in
+    run_codegen (compile_instr me fe (ICase ψ ξ ess)) wl = inr ((), wl', es') ->
+    ⊢ has_type_semantic sr M F L [] (to_e_list es') ψ L'.
+  Admitted.
+
+  Lemma compat_group M F L wl wl' es' τs ρs χ δ κ :
+    let me := me_of_context M mr in
+    let fe := fe_of_context F in
+    Forall2 (fun τ ρ => has_kind F τ (VALTYPE ρ χ δ)) τs ρs ->
+    let τ := ProdT κ τs in
+    has_kind F τ κ ->
+    let ψ := ArrowT τs [τ] in
+    run_codegen (compile_instr me fe (IGroup ψ)) wl = inr ((), wl', es') ->
+    ⊢ has_type_semantic sr M F L [] (to_e_list es') ψ L.
+  Admitted.
+
+  Lemma compat_ungroup M F L wl wl' es' τs ρ χ δ :
+    let me := me_of_context M mr in
+    let fe := fe_of_context F in
+    let κ := VALTYPE ρ χ δ in
+    let τ := ProdT κ τs in
+    has_kind F τ κ ->
+    let ψ := ArrowT [τ] τs in
+    run_codegen (compile_instr me fe (IUngroup ψ)) wl = inr ((), wl', es') ->
+    ⊢ has_type_semantic sr M F L [] (to_e_list es') ψ L.
+  Admitted.
+
+  Lemma compat_fold M F L wl wl' es' τ κ :
+    let me := me_of_context M mr in
+    let fe := fe_of_context F in
+    has_kind F τ κ ->
+    let τ0 := subst_type VarM VarR VarS (unscoped.scons (RecT κ τ) VarT) τ in
+    let ψ := ArrowT [τ0] [RecT κ τ] in
+    run_codegen (compile_instr me fe (IFold ψ)) wl = inr ((), wl', es') ->
+    ⊢ has_type_semantic sr M F L [] (to_e_list es') ψ L.
+  Admitted.
+
+  Lemma compat_unfold M F L wl wl' es' τ κ :
+    let me := me_of_context M mr in
+    let fe := fe_of_context F in
+    let τ0 := subst_type VarM VarR VarS (unscoped.scons (RecT κ τ) VarT) τ in
+    let ψ := ArrowT [RecT κ τ] [τ0] in
+    run_codegen (compile_instr me fe (IUnfold ψ)) wl = inr ((), wl', es') ->
+    ⊢ has_type_semantic sr M F L [] (to_e_list es') ψ L.
+  Admitted.
+
+  Lemma compat_pack M F L wl wl' es' τ τ' :
+    let me := me_of_context M mr in
+    let fe := fe_of_context F in
+    pack_existential_type F τ τ' ->
+    let ψ := ArrowT [τ] [τ'] in
+    run_codegen (compile_instr me fe (IPack ψ)) wl = inr ((), wl', es') ->
+    ⊢ has_type_semantic sr M F L [] (to_e_list es') ψ L.
+  Admitted.
+
+  Lemma compat_unpack_mem M F L wl wl' es es' ξ τ τs1 τs2 κ :
+    let me := me_of_context M mr in
+    let fe := fe_of_context F in
+    let F' := RecordSet.set fc_mem_vars S (subst_function_ctx (up_memory VarM) VarR VarS VarT F) in
+    let L' := update_locals ξ L in
+    let weak := map (subst_type (up_memory VarM) VarR VarS VarT) in
+    instrs_have_type M F' (weak L) es (ArrowT (weak τs1 ++ [τ]) (weak τs2)) (weak L') ->
+    let ψ := ArrowT (τs1 ++ [ExMemT κ τ]) τs2 in
+    (forall wl wl' es',
+        let fe' := fe_of_context F' in
+        run_codegen (compile_instrs me fe' es) wl = inr ((), wl', es') ->
+        ⊢ has_type_semantic sr M F' (weak L) wl'
+          (to_e_list es')
+          (ArrowT (weak τs1 ++ [τ]) (weak τs2)) (weak L')) ->
+    run_codegen (compile_instr me fe (IUnpack ψ ξ es)) wl = inr ((), wl', es') ->
+    ⊢ has_type_semantic sr M F L [] (to_e_list es') ψ L'.
+  Admitted.
+
+  Lemma compat_unpack_rep M F L wl wl' es es' ξ τ τs1 τs2 κ :
+    let me := me_of_context M mr in
+    let fe := fe_of_context F in
+    let F' := RecordSet.set fc_rep_vars S (subst_function_ctx VarM (up_representation VarR) VarS VarT F) in
+    let L' := update_locals ξ L in
+    let weak := map (subst_type VarM (up_representation VarR) VarS VarT) in
+    instrs_have_type M F' (weak L) es (ArrowT (weak τs1 ++ [τ]) (weak τs2)) (weak L') ->
+    let ψ := ArrowT (τs1 ++ [ExRepT κ τ]) τs2 in
+    (forall wl wl' es',
+        let fe' := fe_of_context F' in
+        run_codegen (compile_instrs me fe' es) wl = inr ((), wl', es') ->
+        ⊢ has_type_semantic sr M F' (weak L) wl'
+          (to_e_list es')
+          (ArrowT (weak τs1 ++ [τ]) (weak τs2)) (weak L')) ->
+    run_codegen (compile_instr me fe (IUnpack ψ ξ es)) wl = inr ((), wl', es') ->
+    ⊢ has_type_semantic sr M F L [] (to_e_list es') ψ L'.
+  Admitted.
+
+  Lemma compat_unpack_size M F L wl wl' es es' ξ τ τs1 τs2 κ :
+    let me := me_of_context M mr in
+    let fe := fe_of_context F in
+    let F' := RecordSet.set fc_size_vars S (subst_function_ctx VarM VarR (up_size VarS) VarT F) in
+    let L' := update_locals ξ L in
+    let weak := map (subst_type VarM VarR (up_size VarS) VarT) : list type → list type in
+    instrs_have_type M F' (weak L) es (ArrowT (weak τs1 ++ [τ]) (weak τs2)) (weak L') ->
+    let ψ := ArrowT (τs1 ++ [ExRepT κ τ]) τs2 in
+    (forall wl wl' es',
+        let fe' := fe_of_context F' in
+        run_codegen (compile_instrs me fe' es) wl = inr ((), wl', es') ->
+        ⊢ has_type_semantic sr M F' (weak L) wl'
+          (to_e_list es')
+          (ArrowT (weak τs1 ++ [τ]) (weak τs2)) (weak L')) ->
+    run_codegen (compile_instr me fe (IUnpack ψ ξ es)) wl = inr ((), wl', es') ->
+    ⊢ has_type_semantic sr M F L [] (to_e_list es') ψ L'.
+  Admitted.
+
+  Lemma compat_unpack_type M F L wl wl' es es' ξ τ τs1 τs2 κ κ0 :
+    let me := me_of_context M mr in
+    let fe := fe_of_context F in
+    let F' :=
+      RecordSet.set fc_type_vars (cons κ0) (subst_function_ctx VarM VarR VarS (up_type VarT) F)
+    in
+    let L' := update_locals ξ L in
+    let weak := map (subst_type VarM VarR VarS (up_type VarT)) in
+    instrs_have_type M F' (weak L) es (ArrowT (weak τs1 ++ [τ]) (weak τs2)) (weak L') ->
+    let ψ := ArrowT (τs1 ++ [ExTypeT κ κ0 τ]) τs2 in
+    (forall wl wl' es',
+        let fe' := fe_of_context F' in
+        run_codegen (compile_instrs me fe' es) wl = inr ((), wl', es') ->
+        ⊢ has_type_semantic sr M F' (weak L) wl'
+          (to_e_list es')
+          (ArrowT (weak τs1 ++ [τ]) (weak τs2)) (weak L')) ->
+    run_codegen (compile_instr me fe (IUnpack ψ ξ es)) wl = inr ((), wl', es') ->
+    ⊢ has_type_semantic sr M F L [] (to_e_list es') ψ L'.
+  Admitted.
+
+  Lemma compat_wrap M F L wl wl' es' τ0 ρ0 ρ ιs0 ιs κ :
+    let me := me_of_context M mr in
+    let fe := fe_of_context F in
+    mono_rep ρ0 ιs0 ->
+    mono_rep ρ ιs ->
+    convertible_to ιs0 ιs ->
+    let τ := RepT κ ρ τ0 in
+    has_kind F τ κ ->
+    let ψ := ArrowT [τ0] [τ] in
+    run_codegen (compile_instr me fe (IWrap ψ)) wl = inr ((), wl', es') ->
+    ⊢ has_type_semantic sr M F L [] (to_e_list es') ψ L.
+  Admitted.
+
+  Lemma compat_unwrap M F L wl wl' es' τ0 ρ0 ρ ιs0 ιs κ :
+    let me := me_of_context M mr in
+    let fe := fe_of_context F in
+    mono_rep ρ0 ιs0 ->
+    mono_rep ρ ιs ->
+    convertible_to ιs0 ιs ->
+    let τ := RepT κ ρ τ0 in
+    has_kind F τ κ ->
+    let ψ := ArrowT [τ] [τ0] in
+    run_codegen (compile_instr me fe (IUnwrap ψ)) wl = inr ((), wl', es') ->
+    ⊢ has_type_semantic sr M F L [] (to_e_list es') ψ L.
+  Admitted.
+
+  Lemma compat_ref_new M F L wl wl' es' μ τ0 τ0' κ :
+    let me := me_of_context M mr in
+    let fe := fe_of_context F in
+    mono_mem μ ->
+    stores_as F τ0 τ0' ->
+    let τ := RefT κ μ τ0' in
+    has_kind F τ κ ->
+    let ψ := ArrowT [τ0] [τ] in
+    run_codegen (compile_instr me fe (IRefNew ψ)) wl = inr ((), wl', es') ->
+    ⊢ has_type_semantic sr M F L [] (to_e_list es') ψ L.
+  Admitted.
+
+  Lemma compat_ref_load M F L wl wl' es' μ π τ0 τ0' τs__off ρ δ ιs κ :
+    let me := me_of_context M mr in
+    let fe := fe_of_context F in
+    path_to π τ0 τs__off τ0' ->
+    Forall (mono_sized F) τs__off ->
+    has_kind F τ0' (VALTYPE ρ ImCopy δ) ->
+    mono_rep ρ ιs ->
+    let τ := RefT κ μ τ0 in
+    has_kind F τ κ ->
+    let ψ := ArrowT [τ] [τ; τ0'] in
+    run_codegen (compile_instr me fe (IRefLoad ψ π)) wl = inr ((), wl', es') ->
+    ⊢ has_type_semantic sr M F L [] (to_e_list es') ψ L.
+  Admitted.
+
+  Lemma compat_ref_store M F L wl wl' es' μ π τ0 τs τ__π τᵥ κ :
+    let me := me_of_context M mr in
+    let fe := fe_of_context F in
+    path_to π τ0 τs τ__π ->
+    stores_as F τᵥ τ__π ->
+    has_dropability F τ__π ImDrop ->
+    let τ := RefT κ μ τ0 in
+    has_kind F τ κ ->
+    let ψ := ArrowT [τ; τᵥ] [τ] in
+    run_codegen (compile_instr me fe (IRefStore ψ π)) wl = inr ((), wl', es') ->
+    ⊢ has_type_semantic sr M F L [] (to_e_list es') ψ L.
+  Admitted.
+
+  Lemma compat_ref_mm_store M F L wl wl' es' π τᵥ τᵥ' τₘ τₘ' τ0 τ0' σ n δ κ κ' :
+    let me := me_of_context M mr in
+    let fe := fe_of_context F in
+    stores_as F τᵥ τₘ' ->
+    update_at π τ0 τₘ τ0' τₘ' ->
+    has_kind F τₘ (MEMTYPE (Sized σ) (ConstM MemMM) ImDrop) ->
+    has_kind F τₘ' (MEMTYPE (Sized σ) (ConstM MemMM) δ) ->
+    mono_size σ n ->
+    let τ := RefT κ (ConstM MemMM) τ0 in
+    let τ' := RefT κ' (ConstM MemMM) τ0' in
+    has_kind F τ κ ->
+    has_kind F τ' κ' ->
+    let ψ := ArrowT [τ; τᵥ'] [τ'] in
+    run_codegen (compile_instr me fe (IRefStore ψ π)) wl = inr ((), wl', es') ->
+    ⊢ has_type_semantic sr M F L [] (to_e_list es') ψ L.
+  Admitted.
+
+  Lemma compat_ref_swap M F L wl wl' es' μ π τ0 τs__prefix τₘ τᵥ ρ ιs κ :
+    let me := me_of_context M mr in
+    let fe := fe_of_context F in
+    mono_rep ρ ιs ->
+    path_to π τ0 τs__prefix τₘ ->
+    loads_as F τᵥ τₘ ->
+    Forall (mono_sized F) τs__prefix ->
+    let τ := RefT κ μ τ0 in
+    has_kind F τ κ ->
+    let ψ := ArrowT [τ; τᵥ] [τ; τᵥ] in
+    run_codegen (compile_instr me fe (IRefSwap ψ π)) wl = inr ((), wl', es') ->
+    ⊢ has_type_semantic sr M F L [] (to_e_list es') ψ L.
+  Admitted.
+
+  Lemma compat_ref_mm_swap M F L wl wl' es' π τ0 τ0' τs__prefix τₘ τₘ' τᵥ τᵥ' ρ ιs κ κ' :
+    let me := me_of_context M mr in
+    let fe := fe_of_context F in
+    mono_rep ρ ιs ->
+    path_to π τ0 τs__prefix τₘ ->
+    loads_as F τᵥ τₘ ->
+    stores_as F τᵥ' τₘ' ->
+    update_at π τ0 τₘ τ0' τₘ' ->
+    Forall (mono_sized F) τs__prefix ->
+    let τ := RefT κ (ConstM MemMM) τ0 in
+    let τ' := RefT κ' (ConstM MemMM) τ0' in
+    has_kind F τ κ ->
+    has_kind F τ' κ' ->
+    let ψ := ArrowT [τ; τᵥ'] [τ'; τᵥ] in
+    run_codegen (compile_instr me fe (IRefSwap ψ π)) wl = inr ((), wl', es') ->
+    ⊢ has_type_semantic sr M F L [] (to_e_list es') ψ L.
+  Admitted.
+
+  Lemma compat_nil M F L wl wl' es' :
+    let me := me_of_context M mr in
+    let fe := fe_of_context F in
+    run_codegen (compile_instrs me fe []) es' = inr ((), wl, wl') ->
+    ⊢ has_type_semantic sr M F L wl (to_e_list wl') (ArrowT [] []) L.
+  Admitted.
+
+  Lemma compat_cons M F L1 L2 L3 wl wl' es' e es τs1 τs2 τs3 :
+    let me := me_of_context M mr in
+    let fe := fe_of_context F in
+    instr_has_type M F L1 e (ArrowT τs1 τs2) L2 ->
+    instrs_have_type M F L2 es (ArrowT τs2 τs3) L3 ->
+    (forall es' wl wl',
+        run_codegen (compile_instr me fe e) wl = inr ((), wl', es') ->
+        ⊢ has_type_semantic sr M F L1 [] (to_e_list es') (ArrowT τs1 τs2) L2) ->
+    (forall wl wl' es',
+        run_codegen (compile_instrs me fe es) wl = inr ((), wl', es') ->
+        ⊢ has_type_semantic sr M F L2 wl' (to_e_list es') (ArrowT τs2 τs3) L3) ->
+    run_codegen (compile_instrs me fe (e :: es)) es' = inr ((), wl, wl') ->
+    ⊢ has_type_semantic sr M F L1 wl (to_e_list wl') (ArrowT τs1 τs3) L3.
+  Admitted.
+
+  Theorem fundamental_theorem M F L L' wl wl' es es' tf :
     instrs_have_type M F L es tf L' ->
+    let me := me_of_context M mr in
+    let fe := fe_of_context F in
     run_codegen (compile_instrs me fe es) wl = inr (tt, wl', es') ->
     ⊢ has_type_semantic sr M F L wl' (to_e_list es') tf L'.
   Proof.
-    intros Htyp Hcomp.
+    intros Htype.
     generalize dependent es'.
-    induction Htyp using instrs_have_type_mind with
-      (P := fun C F L e ta L' _ =>
-              forall es',
+    generalize dependent wl'.
+    generalize dependent wl.
+    induction Htype using instrs_have_type_mind with
+      (P := fun M F L e ψ L' _ =>
+              forall es' wl wl',
+                let me := me_of_context M mr in
+                let fe := fe_of_context F in
                 run_codegen (compile_instr me fe e) wl = inr (tt, wl', es') ->
-                ⊢ has_type_semantic sr C F L [] (to_e_list es') ta L');
-    intros es' Hcomp.
-  Admitted.
+                ⊢ has_type_semantic sr M F L [] (to_e_list es') ψ L');
+      intros me fe es' wl wl' Hcomp.
+    - eapply compat_nop; eassumption.
+    - eapply compat_unreachable; eassumption.
+    - eapply compat_copy; eassumption.
+    - eapply compat_drop; eassumption.
+    - eapply compat_num; eassumption.
+    - eapply compat_num_const; eassumption.
+    - eapply compat_block; eassumption.
+    - eapply compat_loop; eassumption.
+    - eapply compat_ite.
+      1: exact Htype1.
+      all: eassumption.
+    - eapply compat_br; eassumption.
+    - eapply compat_br_if; eassumption.
+    - eapply compat_br_table; eassumption.
+    - eapply compat_return; eassumption.
+    - eapply compat_local_get; eassumption.
+    - eapply compat_local_get_copy; eassumption.
+    - eapply compat_local_set; eassumption.
+    - eapply compat_global_get; eassumption.
+    - eapply compat_global_set; eassumption.
+    - eapply compat_global_swap; eassumption.
+    - eapply compat_coderef; eassumption.
+    - eapply compat_inst; eassumption.
+    - eapply compat_call; eassumption.
+    - eapply compat_call_indirect; eassumption.
+    - eapply compat_inject; eassumption.
+    - eapply compat_case; eassumption.
+    - eapply compat_group; eassumption.
+    - eapply compat_ungroup; eassumption.
+    - eapply compat_fold; eassumption.
+    - eapply compat_unfold; eassumption.
+    - eapply compat_pack; eassumption.
+    - eapply compat_unpack_mem; eassumption.
+    - eapply compat_unpack_rep; eassumption.
+    - eapply compat_unpack_size; eassumption.
+    - eapply compat_unpack_type; eassumption.
+    - eapply compat_wrap.
+      1: exact m.
+      all: eassumption.
+    - eapply compat_unwrap.
+      1: exact m.
+      all: eassumption.
+    - eapply compat_ref_new; eassumption.
+    - eapply compat_ref_load; eassumption.
+    - eapply compat_ref_store; eassumption.
+    - eapply compat_ref_mm_store; eassumption.
+    - eapply compat_ref_swap; eassumption.
+    - eapply compat_ref_mm_swap; eassumption.
+    - eapply compat_nil; eassumption.
+    - eapply compat_cons; eassumption.
+  Qed.
 
 End Fundamental.
